designing new syntax and semantics

platform/cito/Dict.v
@@ -12,21 +12,35 @@ End DATA.
 Module Dict (MKey : KEY) (MData : DATA).
 
   Import MKey MData.
+  Definition map := key -> data.
 
-  Definition dict := key -> data.
+  Definition dict := (list key * map)%type.
 
-  Definition upd (m : dict) key value k :=
-    if eq_dec k key then
-      value
-      else
-        m k.
+  Definition upd_map (m : map) k v k' :=
+    if eq_dec k' k then v else m k'.
 
-  Lemma sel_upd_eq : forall m k v k', k' = k ->  upd m k v k' = v.
-    intros; unfold upd; destruct (eq_dec k' k); intuition.
+  Require Import List.
+
+  Definition sel (d : dict) (k : key) : option data.
+    admit.
+  Defined.
+
+  Definition upd (d : dict) k v := ((k :: fst d), upd_map (snd d) k v).
+
+  Definition keys (d : dict) : list key.
+    admit.
+  Defined.
+
+  Definition remove (d : dict) (k : key) : dict.
+    admit.
+  Defined.
+
+  Lemma sel_upd_eq : forall m k v k', k' = k ->  sel (upd m k v) k' = Some v.
+    admit. (*intros; unfold upd; destruct (eq_dec k' k); intuition.*)
   Qed.
 
-  Lemma sel_upd_ne : forall m k v k', k' <> k -> upd m k v k' = m k'.
-    intros; unfold upd; destruct (eq_dec k' k); intuition.
+  Lemma sel_upd_ne : forall m k v k', k' <> k -> sel (upd m k v) k' = sel m k'.
+    admit. (*intros; unfold upd; destruct (eq_dec k' k); intuition.*)
   Qed.
 
 End Dict.
