platform/cito/DepthExpr.v
@@ -1,0 +1,11 @@
+Require Import SyntaxExpr.
+
+(* The depth of stack actually used by compileExpr *)
+Fixpoint depth expr := 
+  match expr with
+    | Var _ => 0
+    | Const _ => 0
+    | Binop _ a b => max (depth a) (S (depth b))
+    | TestE _ a b => max (depth a) (S (depth b))
+  end.
+
